refactor: add ofFnTR

Batteries/Data/List/Basic.lean
@@ -736,15 +736,28 @@ def sigmaTR {σ : α → Type _} (l₁ : List α) (l₂ : ∀ a, List (σ a)) : 
 ofFn f = [f 0, f 1, ... , f (n - 1)]
 ```
 -/
-def ofFn {n} (f : Fin n → α) : List α := go n (Nat.le_refl _) where
-  /-- Auxiliary for `List.ofFn`. -/
-  -- This used to be defined via `Array.ofFn`
-  -- but `Array.ofFn.go` is defined by well-founded recursion (slow to reduce)
-  -- and used `Array.push` (quadratic complexity on lists). Since mathlib relies on
-  -- reducing `List.ofFn`, use a structurally recursive definition here.
-  go : (i : Nat) → (h : i ≤ n) → List α
-  | 0, _ => []
-  | i+1, h => f ⟨n - (i+1), by omega⟩ :: go i (by omega)
+def ofFn {n} (f : Fin n → α) : List α := go n 0 rfl where
+  /-- Auxiliary for `List.ofFn`. `ofFn.go f i j _ = [f j, ..., f (n - 1)]`. -/
+  -- This used to be defined via `Array.ofFn` but mathlib relies on reducing it,
+  -- so we use a structurally recursive definition here.
+  go : (i j : Nat) → (h : i + j = n) → List α
+  | 0, _, _ => []
+  | i+1, j, h => f ⟨j, by omega⟩ :: go i (j+1) (Nat.add_right_comm .. ▸ h :)
+
+/-- Tail-recursive version of `ofFn`. -/
+@[inline] def ofFnTR {n} (f : Fin n → α) : List α := go n (Nat.le_refl _) [] where
+  /-- Auxiliary for `List.ofFnTR`. `ofFnTR.go f i _ acc = f 0 :: ... :: f (i - 1) :: acc`. -/
+  go : (i : Nat) → (h : i ≤ n) → List α → List α
+  | 0, _, acc => acc
+  | i+1, h, acc => go i (Nat.le_of_lt h) (f ⟨i, h⟩ :: acc)
+
+@[csimp] theorem ofFn_eq_ofFnTR : @ofFn = @ofFnTR := by
+  funext α n f; simp [ofFnTR]
+  let rec go (i j h h') : ofFnTR.go f j h' (ofFn.go f i j h) = ofFn f := by
+    unfold ofFnTR.go; split
+    · subst h; rfl
+    · next l j h' => exact go (i+1) j ((Nat.succ_add ..).trans h) (Nat.le_of_lt h')
+  exact (go 0 n (Nat.zero_add _) (Nat.le_refl _)).symm
 
 /-- `ofFnNthVal f i` returns `some (f i)` if `i < n` and `none` otherwise. -/
 def ofFnNthVal {n} (f : Fin n → α) (i : Nat) : Option α :=
